theories/sets.v
@@ -7,6 +7,7 @@ Require Import basics.
 Require Import preord.
 Require Import categories.
 
+Declare Scope set_scope.
 Delimit Scope set_scope with set.
 Open Scope set_scope.
 
