generate_deps.pl
@@ -1,13 +1,6 @@
 print "digraph logrel_deps {\n";
 # See here for color schemes: https://graphviz.org/doc/info/colors.html
 print "  node [shape = ellipse,style=filled,colorscheme = paired12];\n";
-# print "  subgraph cluster_autosubst { label=\"AutoSubst\" \n}";
-# print "  subgraph cluster_syntax { label=\"Syntax\" \n}";
-# print "  subgraph cluster_logrel { label=\"LogicalRelation\" \n}";
-# print "  subgraph cluster_subst { label=\"Validity\" \n}";
-# print "  subgraph cluster_typing { label=\"TypingProperties\" \n}";
-# print "  subgraph cluster_algo { label=\"Algorithmic\" \n}";
-# print "  subgraph cluster_check { label=\"Checkers\" \n}";
 while (<>) {
   if (m/.*?theories\/([^\s]*)\.vo.*:(.*)/) {
     $dests = $2 ;
